PAC_Checker_LLVM/PAC_Checker_Synthesis.thy
@@ -6,7 +6,7 @@
 theory PAC_Checker_Synthesis
   imports PAC_Checker IICF_HashSet PAC_Step_Assn
     PAC_Checker_Init More_Loops LLVM_String
-    IICF_PartialMap
+    IICF_PartialMap PAC_Checker_Relation
 begin
 
 section \<open>Code Synthesis of the Complete Checker\<close>
@@ -231,13 +231,26 @@ lemma union_vars_poly_alt_def:
      (auto simp: vars_llist_def union_vars_monom_alt_def)
    done
 
-type_synonym status_conc = \<open>8 word \<times> strl_conc\<close>
+term stra_assn
+type_synonym stra_conc = \<open>64 word \<times> 8 word ptr\<close>
+type_synonym status_conc = \<open>8 word \<times> stra_conc\<close>
+
+definition msg_assn :: \<open>string \<Rightarrow> stra_conc \<Rightarrow> assn\<close> where
+  \<open>msg_assn s si \<equiv> stra_assn (capped s) si\<close>
+
+lemma msg_assn_capped[simp]: \<open>msg_assn (capped s) = msg_assn s\<close>
+  unfolding msg_assn_def by simp
+
+lemma msg_assn_mk_free[sepref_frame_free_rules]: \<open>MK_FREE msg_assn la_free_impl\<close>
+  apply (rule MK_FREEI)
+  unfolding msg_assn_def
+  by (rule MK_FREED[OF larray_mk_free])
 
 definition status_assn :: \<open>string code_status \<Rightarrow> status_conc \<Rightarrow> assn\<close> where
   \<open>status_assn c \<equiv> \<lambda>(tag,msgi). case c of
     CSUCCESS    \<Rightarrow> \<up>(tag = 0) ** \<box>
   | CFOUND      \<Rightarrow> \<up>(tag = 1) ** \<box>
-  | CFAILED msg \<Rightarrow> \<up>(tag = 2) ** strl_assn' msg msgi
+  | CFAILED msg \<Rightarrow> \<up>(tag = 2) ** msg_assn msg msgi
   \<close>
 
 lemma status_assn_csuccess_conv[simp]:
@@ -249,8 +262,26 @@ lemma status_assn_cfound_conv[simp]:
   unfolding status_assn_def by simp
 
 lemma status_assn_cfailed_conv[simp]:
-  \<open>status_assn (CFAILED msg) (tag, msgi) \<equiv> \<up>(tag = 2) ** strl_assn' msg msgi\<close>
+  \<open>status_assn (CFAILED msg) (tag, msgi) \<equiv> \<up>(tag = 2) ** msg_assn msg msgi\<close>
   unfolding status_assn_def by simp
+
+lemma status_assn_capped[simp]: \<open>status_assn (CFAILED (capped msg)) = status_assn (CFAILED msg)\<close>
+  by (intro ext) (auto simp: status_assn_def split: prod.splits)
+
+text \<open>The tag is determined by the discriminators. Stating this once keeps the discriminator
+  implementations free of a case split on @{typ \<open>string code_status\<close>}: unfolding
+  @{thm status_assn_def} in those proofs leaves a @{term case_code_status} applied to a state,
+  which the simplifier will not split.\<close>
+lemma status_assn_tagD:
+  assumes \<open>status_assn c (tag, msgi) s\<close>
+  shows \<open>tag = (if is_cfailed c then 2 else if is_cfound c then 1 else 0)\<close>
+proof -
+  have \<open>pure_part (status_assn c (tag, msgi))\<close>
+    using assms by (rule pure_partI)
+  then show ?thesis
+    by (cases c)
+      (auto simp: status_assn_def dest!: pure_part_split_conj pure_part_pureD)
+qed
 
 definition mk_csuccess_impl :: \<open>status_conc llM\<close> where [llvm_code,llvm_inline]:
   \<open>mk_csuccess_impl \<equiv> Mreturn (0, init)\<close>
@@ -259,8 +290,8 @@ definition mk_cfound_impl :: \<open>status_conc llM\<close> where [llvm_code,llv
   \<open>mk_cfound_impl \<equiv> Mreturn (1, init)\<close>
 
 definition mk_cfailed_impl :: \<open>strl_conc \<Rightarrow> status_conc llM\<close> where [llvm_code,llvm_inline]:
-  \<open>mk_cfailed_impl msg \<equiv> Mreturn (2, msg)\<close>
-  
+  \<open>mk_cfailed_impl msg \<equiv> doM { msg' \<leftarrow> stra_of_strl_impl msg; Mreturn (2, msg') }\<close>
+
 lemma SUCCESS_hnr[sepref_fr_rules]:
   \<open>(uncurry0 (mk_csuccess_impl), uncurry0 (RETURN CSUCCESS))
   \<in> unit_assn\<^sup>k \<rightarrow>\<^sub>a status_assn\<close>
@@ -278,12 +309,12 @@ lemma FOUND_hnr[sepref_fr_rules]:
   by (auto simp: sep_algebra_simps ENTAILS_def entails_def)
 
 lemma FAILED_hnr[sepref_fr_rules]:
-  \<open>(mk_cfailed_impl, RETURN o CFAILED)
-  \<in> strl_assn'\<^sup>d \<rightarrow>\<^sub>a status_assn\<close>
+  \<open>(mk_cfailed_impl, RETURN o CFAILED) \<in> strl_assn'\<^sup>d \<rightarrow>\<^sub>a status_assn\<close>
   unfolding mk_cfailed_impl_def
-  apply (sepref_to_hoare)
+  apply sepref_to_hoare
   apply vcg
-  by (auto simp: sep_algebra_simps ENTAILS_def entails_def)
+  by (auto simp: sep_algebra_simps ENTAILS_def entails_def msg_assn_def
+    invalid_assn_def)
 
 (* definition is_csuccess_impl :: \<open>status_conc \<Rightarrow> 1 word llM\<close> where[llvm_code,llvm_inline]:
  *   \<open>is_csuccess_impl \<equiv> \<lambda>(tag,msg). ll_icmp_eq tag 0\<close> *)
@@ -298,24 +329,20 @@ interpretation llvm_prim_arith_setup + llvm_prim_ctrl_setup .
 lemma is_success_hnr[sepref_fr_rules]:
   \<open>(is_cfound_impl, (RETURN o is_cfound))
   \<in> status_assn\<^sup>k \<rightarrow>\<^sub>a bool1_assn\<close>
-  unfolding is_cfound_impl_def is_cfound_def 
+  unfolding is_cfound_impl_def
   apply (sepref_to_hoare; vcg)
-  apply (auto simp: sep_algebra_simps ENTAILS_def entails_def
-    bool1_rel_def bool.rel_def in_br_conv)
-  subgoal for status by (cases status; simp)
-  done
+  by (auto simp: sep_algebra_simps ENTAILS_def entails_def
+    bool1_rel_def bool.rel_def in_br_conv pred_lift_extract_simps
+    dest!: status_assn_tagD split: if_splits)
 
 lemma is_cfailed_hnr[sepref_fr_rules]:
   \<open>(is_cfailed_impl, (RETURN o is_cfailed))
   \<in> status_assn\<^sup>k \<rightarrow>\<^sub>a bool1_assn\<close>
   unfolding is_cfailed_impl_def
   apply (sepref_to_hoare; vcg)
-  apply (simp add: sep_algebra_simps ENTAILS_def entails_def
-    bool1_rel_def bool.rel_def in_br_conv)
-  subgoal for status
-    by (cases status)
-      (auto simp: pred_lift_extract_simps)
-  done
+  by (auto simp: sep_algebra_simps ENTAILS_def entails_def
+    bool1_rel_def bool.rel_def in_br_conv pred_lift_extract_simps
+    dest!: status_assn_tagD split: if_splits)
 
 definition merge_cstatus_impl :: \<open>status_conc \<Rightarrow> status_conc \<Rightarrow> status_conc llM\<close>
   where[llvm_code]: \<open>merge_cstatus_impl \<equiv> \<lambda>(t1,msg1) (t2,msg2). doM {
@@ -324,7 +351,7 @@ definition merge_cstatus_impl :: \<open>status_conc \<Rightarrow> status_conc \<
       (doM {
         failed2 \<leftarrow> is_cfailed_impl (t2,msg2);
         llc_if failed2
-          (doM { strl.cl_free msg2; Mreturn (t1,msg1) })
+          (doM { la_free_impl msg2; Mreturn (t1,msg1) })
           (Mreturn (t1,msg1))
       })
       (doM {
@@ -348,28 +375,19 @@ definition merge_cstatus_impl :: \<open>status_conc \<Rightarrow> status_conc \<
 lemma merge_cstatus_hnr[sepref_fr_rules]:
   \<open>(uncurry merge_cstatus_impl, uncurry (RETURN oo merge_cstatus)) \<in>
     status_assn\<^sup>d *\<^sub>a  status_assn\<^sup>d \<rightarrow>\<^sub>a status_assn\<close>
+  supply [vcg_rules] = msg_assn_mk_free[THEN MK_FREED]
   unfolding merge_cstatus_impl_def is_cfailed_impl_def is_cfound_impl_def
   apply sepref_to_hoare
   subgoal for y x yi xi
     apply (cases x; cases y; cases xi; cases yi; simp)
-    by (all \<open>vcg\<close>)
-      (auto simp: ENTAILS_def entails_def sep_algebra_simps
-        pred_lift_extract_simps sep_conj_exists)
+    apply (all \<open>vcg\<close>)
+    apply (auto simp: ENTAILS_def entails_def sep_algebra_simps
+      pred_lift_extract_simps sep_conj_exists)
   done
 
 end
 
-
-lemma term_order_rel_alt_def:
-  \<open>term_order_rel = lexord (p2rel char.lexordp)\<close>
-  by (auto simp: p2rel_def char.lexordp_conv_lexord var_order_rel_def intro!: arg_cong[of _ _ lexord])
-
-lemma term_order_rel_by_lt: \<open>(x,y) \<in> term_order_rel \<equiv> x < y\<close>
-  by (rule eq_reflection)
-    (auto simp: lexordp_conv_lexord less_eq_list_def less_list_def lexordp_def
-      var_order_rel_def rel2p_def term_order_rel_alt_def p2rel_def less_char_inst)
-
-sepref_definition add_poly_l_impl is \<open>uncurry add_poly_l\<close>
+sepref_def add_poly_l_impl is \<open>uncurry add_poly_l\<close>
   :: \<open>polynomial_assn\<^sup>k *\<^sub>a polynomial_assn\<^sup>k \<rightarrow>\<^sub>a polynomial_assn\<close>
   unfolding add_poly_l_def add_poly_l1_def add_poly_l2_def
     apl_cond_def apl_body_def apl2_body_def ls_emp term_order_rel_by_lt
@@ -379,7 +397,6 @@ lemma var_order_rel_alt: \<open>(x,y) \<in> var_order_rel \<equiv> x < y\<close>
   unfolding var_order_rel_def less_char_def p2rel_def
   by (simp add: List.lexordp_def less_char_def less_char_inst
     less_list_def)
-
 
 definition \<open>mult_monoms_inner p\<^sub>0 q\<^sub>0 \<equiv> WHILEIT
     (\<lambda>(r,p,q). mult_monoms p\<^sub>0 q\<^sub>0 = r @ mult_monoms p q)
@@ -591,7 +608,7 @@ sepref_def mult_poly_impl
 declare mult_poly_impl.refine[sepref_fr_rules]
 
 sepref_register \<open>(=) :: llist_polynomial \<Rightarrow> llist_polynomial \<Rightarrow> bool\<close>
-sepref_definition weak_equality_l_impl
+sepref_def weak_equality_l_impl
   is \<open>uncurry weak_equality_l\<close>
   :: \<open>polynomial_assn\<^sup>k *\<^sub>a polynomial_assn\<^sup>k \<rightarrow>\<^sub>a bool1_assn\<close>
   unfolding weak_equality_l_def
@@ -611,7 +628,7 @@ definition error_msg_not_equal_dom_nres where
               qs @ cl_to_clt '' = '' @
               pqs @ cl_to_clt '' not equal'' @
               rs;
-    RETURN (op_clt_to_cl res)
+    RETURN res
   }\<close> 
 
 term raw_string_assn
@@ -619,7 +636,7 @@ term stra_assn
 
 sepref_register stra_of_strl
 sepref_def error_msg_not_equal_dom_impl is \<open>uncurry3 (error_msg_not_equal_dom_nres)\<close>
-  :: \<open>polynomial_assn\<^sup>k *\<^sub>a polynomial_assn\<^sup>k *\<^sub>a polynomial_assn\<^sup>k *\<^sub>a polynomial_assn\<^sup>k \<rightarrow>\<^sub>a strl_assn'\<close>
+  :: \<open>polynomial_assn\<^sup>k *\<^sub>a polynomial_assn\<^sup>k *\<^sub>a polynomial_assn\<^sup>k *\<^sub>a polynomial_assn\<^sup>k \<rightarrow>\<^sub>a strlt_assn\<close>
   unfolding error_msg_not_equal_dom_nres_def
   by sepref
 
@@ -633,10 +650,10 @@ lemmas error_msg_not_equal_dom_hnr[sepref_fr_rules] =
   error_msg_not_equal_dom_impl.refine[FCOMP error_msg_not_equal_dom_nres_refine]
 
 (* TODO cleanup this section *)
-definition \<open>show_nres \<equiv> chars_of_int o COPY\<close>
+definition \<open>show_nres \<equiv> cl_to_clt o chars_of_int o COPY\<close>
 
 sepref_def show_impl is \<open>RETURN o show_nres\<close>
-  :: \<open>sbi_assn\<^sup>k \<rightarrow>\<^sub>a strl_assn'\<close>
+  :: \<open>sbi_assn\<^sup>k \<rightarrow>\<^sub>a strlt_assn\<close>
   unfolding show_nres_def
   by sepref 
 
@@ -665,9 +682,13 @@ lemma chars_of_int_show: \<open>chars_of_int i = show i\<close>
   by (auto simp: chars_of_int_def shows_prec_int_def showsp_int_def
       showsp_nat_chars_of_nat shows_string_def ascii_hyphen_def)
 
+lemma cl_to_clt_id: \<open>cl_to_clt = id\<close>
+  unfolding cl_to_clt_def
+  by (metis (mono_tags, lifting) append.simps(1) eq_id_iff foldl_snoc)
+    
 lemma show_nres_spec: \<open>(RETURN o show_nres, RETURN o show)
   \<in> Id \<rightarrow>\<^sub>f \<langle>Id\<rangle>nres_rel\<close>
-  unfolding show_nres_def
+  unfolding show_nres_def cl_to_clt_id id_def
   apply (intro frefI nres_relI)
   using chars_of_int_show by auto
 
@@ -676,12 +697,10 @@ definition show_int :: \<open>int \<Rightarrow> string\<close> where
 
 lemma show_nres_int_spec: \<open>(RETURN o show_nres, RETURN o show_int)
   \<in> Id \<rightarrow>\<^sub>f \<langle>Id\<rangle>nres_rel\<close>
-  unfolding show_nres_def show_int_def
+  unfolding show_nres_def show_int_def cl_to_clt_id
   apply (intro frefI nres_relI)
   apply (auto simp: chars_of_int_show)
   done
-
-sepref_register show_int
 
 lemmas show_nres_hnr[sepref_fr_rules] =
   show_impl.refine[FCOMP show_nres_int_spec]
@@ -690,36 +709,48 @@ lemma show_nat_show_int_of_nat: \<open>show (n :: nat) = show_int (of_nat n)\<cl
   unfolding show_int_def chars_of_int_show[symmetric] chars_of_int_def
   by (simp add: shows_prec_nat_def showsp_nat_chars_of_nat)
 
+definition show_nat :: \<open>nat \<Rightarrow> string\<close> where \<open>show_nat \<equiv> show\<close>
+
+sepref_def show_nat_impl is \<open>RETURN o show_nat\<close>
+  :: \<open>si64_assn\<^sup>k \<rightarrow>\<^sub>a strlt_assn\<close>
+  unfolding show_nat_def show_nat_show_int_of_nat
+  by sepref
+
 sepref_register \<open>error_msg_notin_dom :: nat \<Rightarrow> string\<close>
   \<open>error_msg_reused_dom :: nat \<Rightarrow> string\<close>
   \<open>error_msg :: nat \<Rightarrow> string \<Rightarrow> string code_status\<close>
   \<open>CFAILED :: string \<Rightarrow> string code_status\<close>
 
 lemma error_msg_notin_dom_alt:
-  \<open>error_msg_notin_dom i = show_int (of_nat i) @ '' notin domain''\<close>
-  by (simp add: error_msg_notin_dom_def error_msg_notin_dom_err_def show_nat_show_int_of_nat)
+  \<open>error_msg_notin_dom i = show_nat i @ cl_to_clt '' notin domain''\<close>
+  by (simp add: error_msg_notin_dom_def error_msg_notin_dom_err_def show_nat_show_int_of_nat cl_to_clt_def
+    show_nat_def)
 
 sepref_def error_msg_notin_dom_impl is \<open>RETURN o error_msg_notin_dom\<close>
-  :: \<open>si64_assn\<^sup>k \<rightarrow>\<^sub>a strl_assn'\<close>
-  unfolding error_msg_notin_dom_alt[abs_def]
+  :: \<open>si64_assn\<^sup>k \<rightarrow>\<^sub>a strlt_assn\<close>
+  unfolding error_msg_notin_dom_alt
   by sepref
 
 lemma error_msg_reused_dom_alt:
-  \<open>error_msg_reused_dom (i :: nat) = show_int (of_nat i) @ '' already in domain''\<close>
-  by (simp add: error_msg_reused_dom_def show_nat_show_int_of_nat)
+  \<open>error_msg_reused_dom (i :: nat) = show_nat i @ cl_to_clt '' already in domain''\<close>
+  by (simp add: error_msg_reused_dom_def show_nat_def cl_to_clt_id)
 
 sepref_def error_msg_reused_dom_impl is \<open>RETURN o error_msg_reused_dom\<close>
-  :: \<open>si64_assn\<^sup>k \<rightarrow>\<^sub>a strl_assn'\<close>
+  :: \<open>si64_assn\<^sup>k \<rightarrow>\<^sub>a strlt_assn\<close>
   unfolding error_msg_reused_dom_alt[abs_def]
   by sepref
 
+text \<open>No \<open>nres\<close> detour and no \<open>fref\<close> is needed: the program stays the exact abstract
+  @{term error_msg}, and the conversion to the array representation (including its
+  truncation) happens inside @{thm FAILED_hnr}.\<close>
 lemma error_msg_alt:
   \<open>error_msg (i :: nat) msg =
-     CFAILED (''s CHECKING failed at line '' @ show_int (of_nat i) @ '' with error '' @ msg)\<close>
-  by (simp add: error_msg_def show_nat_show_int_of_nat)
+    CFAILED (op_clt_to_cl (cl_to_clt ''s CHECKING failed at line '' @ show_nat i
+                         @ cl_to_clt '' with error '' @ msg))\<close>
+  by (simp add: error_msg_def cl_to_clt_id show_nat_def show_nat_show_int_of_nat)
 
 sepref_def error_msg_impl is \<open>uncurry (RETURN oo error_msg)\<close>
-  :: \<open>si64_assn\<^sup>k *\<^sub>a strl_assn'\<^sup>d \<rightarrow>\<^sub>a status_assn\<close>
+  :: \<open>si64_assn\<^sup>k *\<^sub>a strlt_assn\<^sup>d \<rightarrow>\<^sub>a status_assn\<close>
   unfolding error_msg_alt[abs_def]
   by sepref
 
@@ -733,39 +764,94 @@ interpretation polys: boxed_copying_pmap
 abbreviation polys_assn where
   \<open>polys_assn \<equiv> hr_comp (hr_comp polys.bx.pmap_assn' opt_list_map_rel) map_fmap_rel\<close>
 
-term check_addition_l
-sepref_definition check_addition_l_impl
+lemma polys_assn_intf[intf_of_assn]:
+  \<open>intf_of_assn polys_assn TYPE((nat, (char list list \<times> int) list) f_map)\<close>
+  by simp
+
+(* These lemmas used to exist similarly in PAC_Map_Rel.thy *)
+lemmas fmap_empty_hnr[sepref_fr_rules] =
+  polys.bx.pmap_empty_hnr2[FCOMP fmempty_empty]
+
+lemmas fmap_delete_hnr[sepref_fr_rules] =
+  polys.bx.pmap_delete_hnr2[FCOMP fmdrop_set_None]
+
+lemmas fmap_update_hnr[sepref_fr_rules] =
+  polys.bx.pmap_update_hnr2[FCOMP map_upd_fmupd]
+
+lemmas fmap_lookup_hnr[sepref_fr_rules] =
+  polys.bx.cpmap_lookup_hnr2[FCOMP op_map_lookup_fmlookup]
+
+sepref_register fmlookup' :: \<open>'k \<Rightarrow> ('k, 'v) f_map \<Rightarrow> 'v option\<close>
+
+lemma map_fmap_contains_key:
+  \<open>(uncurry (RETURN oo op_map_contains_key), uncurry (RETURN oo op_fmap_contains_key))
+     \<in> Id \<times>\<^sub>r map_fmap_rel \<rightarrow>\<^sub>f \<langle>bool_rel\<rangle>nres_rel\<close>
+  by (intro frefI nres_relI)
+    (auto simp: op_map_contains_key_def op_fmap_contains_key_def map_fmap_rel_def
+      br_def in_fdom_alt fmap.Abs_fmap_inverse split: option.splits)
+
+lemmas fmap_contains_key_hnr[sepref_fr_rules] =
+  polys.bx.pmap_contains_key_hnr2[FCOMP map_fmap_contains_key]
+
+lemma in_dom_by_contains: \<open>k\<in># dom_m A = op_fmap_contains_key k A\<close>
+  unfolding op_fmap_contains_key_def by simp
+
+sepref_decl_op fmap_the_lookup: \<open>\<lambda>k m. the (fmlookup' k m)\<close>
+  :: \<open>[\<lambda>(k, m). k \<in># dom_m m]\<^sub>f K \<times>\<^sub>r \<langle>K,V\<rangle>fmap_rel \<rightarrow> V\<close>
+  using fmap_rel_in_dom_iff by fastforce
+
+(* lemma the_lookup_alt:
+ *   \<open>the (fmlookup' k m) = UNBOX (op_fmap_the_lookup k m)\<close>
+ *   by simp *)
+
+lemma op_the_lookup_refine:
+  \<open>(uncurry (RETURN oo op_map_the_lookup), uncurry (RETURN oo op_fmap_the_lookup))
+     \<in> [\<lambda>(k, m). k \<in># dom_m m]\<^sub>f Id \<times>\<^sub>r map_fmap_rel \<rightarrow> \<langle>Id\<rangle>nres_rel\<close>
+  apply (intro frefI nres_relI)
+  by (auto simp: map_fmap_rel_def br_def in_fdom_alt fmap.Abs_fmap_inverse)
+
+lemma map_fmap_rel_dom_iff[fcomp_prenorm_simps]:
+  \<open>(m, fm) \<in> map_fmap_rel \<Longrightarrow> (\<exists>y. m k = Some y) \<longleftrightarrow> k \<in># dom_m fm\<close>
+  by (auto simp: map_fmap_rel_def br_def in_fdom_alt fmap.Abs_fmap_inverse)
+
+lemmas fmap_the_lookup_hnr[sepref_fr_rules] =
+  polys.bx.cpmap_the_lookup_hnr2[FCOMP op_the_lookup_refine]
+
+lemma pat_fmap_the_lookup[def_pat_rules]:
+  \<open>the$(fmlookup'$k$m) \<equiv> UNBOX$(op_fmap_the_lookup$k$m)\<close>
+  by (simp add: UNBOX_def)
+
+term error_msg
+sepref_def check_addition_l_impl
   is \<open>uncurry6 check_addition_l\<close>
   :: \<open>polynomial_assn\<^sup>k *\<^sub>a polys_assn\<^sup>k *\<^sub>a vars_assn\<^sup>k *\<^sub>a
   si64_assn\<^sup>k *\<^sub>a si64_assn\<^sup>k *\<^sub>a si64_assn\<^sup>k *\<^sub>a polynomial_assn\<^sup>k
   \<rightarrow>\<^sub>a status_assn\<close>
   supply [[goals_limit=1]]
-    thm fmlookup'_def[symmetric]
   unfolding
-    mult_poly_full_def
     check_addition_l_def
+    mult_poly_full_def
     vars_llist_alt_def
-    in_dom_m_lookup_iff
-
-  apply sepref_dbg_keep
-  apply sepref_dbg_trans_keep
-  apply sepref_dbg_trans_step_keep
-  apply sepref_dbg_side_unfold
-
-
-declare check_addition_l_impl.refine[sepref_fr_rules]
+    fmlookup'_def[symmetric]
+    in_dom_by_contains
+    fold_clt_empty
+  by sepref
 
 sepref_register check_mult_l_dom_err
 
+thm show_nat_show_int_of_nat
 definition check_mult_l_dom_err_imp where
   \<open>check_mult_l_dom_err_imp pd p ia i =
-    (if pd then ''The polynomial with id '' @ show p @ '' was not found'' else '''') @
-    (if ia then ''The id of the resulting id '' @ show i @ '' was already given'' else '''')\<close>
+    (if pd then (cl_to_clt ''The polynomial with id '')
+                 @ show_nat p
+                 @ (cl_to_clt '' was not found'') else op_clt_empty) @
+    (if ia then (cl_to_clt ''The id of the resulting id '')
+                 @ show_nat i
+                 @ (cl_to_clt '' was already given'') else op_clt_empty)\<close>
 
 sepref_def check_mult_l_dom_err_impl is \<open>uncurry3 (RETURN oooo check_mult_l_dom_err_imp)\<close>
-  :: \<open>bool1_assn\<^sup>k *\<^sub>a si64_assn\<^sup>k *\<^sub>a bool1_assn\<^sup>k *\<^sub>a si64_assn\<^sup>k \<rightarrow>\<^sub>a strl_assn'\<close>
-  unfolding check_mult_l_dom_err_imp_def
-    show_nat_show_int_of_nat
+  :: \<open>bool1_assn\<^sup>k *\<^sub>a si64_assn\<^sup>k *\<^sub>a bool1_assn\<^sup>k *\<^sub>a si64_assn\<^sup>k \<rightarrow>\<^sub>a strlt_assn\<close>
+  unfolding check_mult_l_dom_err_imp_def 
   by sepref
 
 lemma check_mult_l_dom_err_imp_spec:
@@ -780,160 +866,284 @@ lemma check_mult_l_dom_err_imp_spec:
 lemmas check_mult_l_dom_err_impl_hnr[sepref_fr_rules] =
   check_mult_l_dom_err_impl.refine[FCOMP check_mult_l_dom_err_imp_spec]
 
+thm poly_print_hnr
 definition check_mult_l_mult_err_imp where
   \<open>check_mult_l_mult_err_imp p q pq r =
-    ''Multiplying '' @ show p @ '' by '' @ show q @ '' gives '' @ show pq @ '' and not '' @ show r\<close>
+  cl_to_clt ''Multiplying '' @ poly_print p @ cl_to_clt '' by '' @ poly_print q @
+  cl_to_clt '' gives '' @ poly_print pq @ cl_to_clt '' and not '' @ poly_print r\<close>
 
-lemma [sepref_fr_rules]:
-  \<open>(uncurry3 ((\<lambda>x y. return oo (check_mult_l_mult_err_impl x y))),
-   uncurry3 (check_mult_l_mult_err)) \<in> poly_assn\<^sup>k *\<^sub>a poly_assn\<^sup>k *\<^sub>a poly_assn\<^sup>k *\<^sub>a poly_assn\<^sup>k \<rightarrow>\<^sub>a raw_string_assn\<close>
-   unfolding check_mult_l_mult_err_def check_mult_l_mult_err_impl_def list_assn_pure_conv
-   apply sepref_to_hoare
-   apply sep_auto
-   done
+sepref_def check_mult_l_mult_err_impl is
+  \<open>uncurry3 (RETURN oooo check_mult_l_mult_err_imp)\<close> ::
+  \<open>polynomial_assn\<^sup>k *\<^sub>a polynomial_assn\<^sup>k *\<^sub>a polynomial_assn\<^sup>k *\<^sub>a polynomial_assn\<^sup>k
+  \<rightarrow>\<^sub>a strlt_assn\<close>
+  unfolding check_mult_l_mult_err_imp_def
+  by sepref
 
-sepref_definition check_mult_l_impl
+lemma check_mult_l_mult_err_imp_spec:
+  \<open>(uncurry3 (RETURN oooo check_mult_l_mult_err_imp),
+  uncurry3 check_mult_l_mult_err) \<in> Id \<rightarrow>\<^sub>f \<langle>Id\<rangle>nres_rel\<close>
+  apply (intro frefI nres_relI)
+  unfolding check_mult_l_mult_err_imp_def
+    cl_to_clt_id check_mult_l_mult_err_def
+  by auto 
+
+lemmas check_mult_l_mult_err_hnr[sepref_fr_rules] = 
+  check_mult_l_mult_err_impl.refine[FCOMP check_mult_l_mult_err_imp_spec]
+
+sepref_register check_mult_l_mult_err
+sepref_def check_mult_l_impl
   is \<open>uncurry6 check_mult_l\<close>
-  :: \<open>poly_assn\<^sup>k *\<^sub>a polys_assn\<^sup>k *\<^sub>a vars_assn\<^sup>k *\<^sub>a uint64_nat_assn\<^sup>k *\<^sub>a poly_assn\<^sup>k *\<^sub>a uint64_nat_assn\<^sup>k *\<^sub>a poly_assn\<^sup>k  \<rightarrow>\<^sub>a status_assn raw_string_assn\<close>
+  :: \<open>polynomial_assn\<^sup>k *\<^sub>a polys_assn\<^sup>k *\<^sub>a vars_assn\<^sup>k *\<^sub>a
+  si64_assn\<^sup>k *\<^sub>a polynomial_assn\<^sup>k *\<^sub>a si64_assn\<^sup>k *\<^sub>a polynomial_assn\<^sup>k  \<rightarrow>\<^sub>a status_assn\<close>
   supply [[goals_limit=1]]
   unfolding check_mult_l_def
-    HOL_list.fold_custom_empty
     term_order_rel'_def[symmetric]
     term_order_rel'_alt_def
-    in_dom_m_lookup_iff
+    in_dom_by_contains
     fmlookup'_def[symmetric]
     vars_llist_alt_def
   by sepref
 
-declare check_mult_l_impl.refine[sepref_fr_rules]
 
-definition check_ext_l_dom_err_impl :: \<open>uint64 \<Rightarrow> _\<close>  where
-  \<open>check_ext_l_dom_err_impl p =
-    ''There is already a polynomial with index '' @ show (nat_of_uint64 p)\<close>
+definition check_ext_l_dom_err_imp :: \<open>nat \<Rightarrow> _\<close>  where
+  \<open>check_ext_l_dom_err_imp p =
+    cl_to_clt ''There is already a polynomial with index '' @ show_nat p\<close>
 
-lemma [sepref_fr_rules]:
-  \<open>(((return o (check_ext_l_dom_err_impl))),
-    (check_extension_l_dom_err)) \<in> uint64_nat_assn\<^sup>k \<rightarrow>\<^sub>a raw_string_assn\<close>
-   unfolding check_extension_l_dom_err_def check_ext_l_dom_err_impl_def list_assn_pure_conv
-   apply sepref_to_hoare
-   apply sep_auto
-   done
+sepref_def check_ext_l_dom_err_impl is \<open>RETURN o check_ext_l_dom_err_imp\<close>
+  :: \<open>si64_assn\<^sup>k \<rightarrow>\<^sub>a strlt_assn\<close>
+  unfolding check_ext_l_dom_err_imp_def
+  by sepref
 
+lemma check_ext_l_dom_err_spec: 
+  \<open>(RETURN o check_ext_l_dom_err_imp, check_extension_l_dom_err)
+  \<in> Id \<rightarrow>\<^sub>f \<langle>Id\<rangle>nres_rel\<close>
+  apply (intro frefI nres_relI)
+  unfolding check_ext_l_dom_err_imp_def check_extension_l_dom_err_def
+  by auto 
 
-definition check_extension_l_no_new_var_err_impl :: \<open>_ \<Rightarrow> _\<close>  where
-  \<open>check_extension_l_no_new_var_err_impl p =
-    ''No new variable could be found in polynomial '' @ show p\<close>
+lemmas check_ext_l_dom_err_hnr[sepref_fr_rules] =
+  check_ext_l_dom_err_impl.refine[FCOMP check_ext_l_dom_err_spec]
 
-lemma [sepref_fr_rules]:
-  \<open>(((return o (check_extension_l_no_new_var_err_impl))),
-    (check_extension_l_no_new_var_err)) \<in> poly_assn\<^sup>k \<rightarrow>\<^sub>a raw_string_assn\<close>
-   unfolding check_extension_l_no_new_var_err_impl_def check_extension_l_no_new_var_err_def
-     list_assn_pure_conv
-   apply sepref_to_hoare
-   apply sep_auto
-   done
+definition check_extension_l_no_new_var_err_imp :: \<open>llist_polynomial \<Rightarrow> string\<close>  where
+  \<open>check_extension_l_no_new_var_err_imp p =
+    cl_to_clt ''No new variable could be found in polynomial '' @ poly_print p\<close>
 
-definition check_extension_l_side_cond_err_impl :: \<open>_ \<Rightarrow> _\<close>  where
-  \<open>check_extension_l_side_cond_err_impl v p r s =
-    ''Error while checking side conditions of extensions polynow, var is '' @ show v @
-    '' polynomial is '' @ show p @ ''side condition p*p - p = '' @ show s @ '' and should be 0''\<close>
+sepref_def check_extension_l_no_new_var_err_impl is \<open>RETURN o check_extension_l_no_new_var_err_imp\<close> 
+  :: \<open>polynomial_assn\<^sup>k \<rightarrow>\<^sub>a strlt_assn\<close>
+  unfolding check_extension_l_no_new_var_err_imp_def
+  by sepref
 
-lemma [sepref_fr_rules]:
-  \<open>((uncurry3 (\<lambda>x y. return oo (check_extension_l_side_cond_err_impl x y))),
-    uncurry3 (check_extension_l_side_cond_err)) \<in> string_assn\<^sup>k *\<^sub>a poly_assn\<^sup>k *\<^sub>a poly_assn\<^sup>k *\<^sub>a poly_assn\<^sup>k \<rightarrow>\<^sub>a raw_string_assn\<close>
-   unfolding check_extension_l_side_cond_err_impl_def check_extension_l_side_cond_err_def
-     list_assn_pure_conv
-   apply sepref_to_hoare
-   apply sep_auto
-   done
+lemma check_extension_l_no_new_var_err_spec:
+  \<open>(RETURN o check_extension_l_no_new_var_err_imp,
+    check_extension_l_no_new_var_err) \<in> Id \<rightarrow>\<^sub>f \<langle>Id\<rangle>nres_rel\<close>
+  apply (intro frefI nres_relI)
+  unfolding check_extension_l_no_new_var_err_imp_def
+    check_extension_l_no_new_var_err_def
+  by auto
 
-definition check_extension_l_new_var_multiple_err_impl :: \<open>_ \<Rightarrow> _\<close>  where
-  \<open>check_extension_l_new_var_multiple_err_impl v p =
-    ''Error while checking side conditions of extensions polynow, var is '' @ show v @
-    '' but it either appears at least once in the polynomial or another new variable is created '' @
-    show p @ '' but should not.''\<close>
+lemmas check_extension_l_no_new_var_err_hnr[sepref_fr_rules] =
+  check_extension_l_no_new_var_err_impl.refine[FCOMP check_extension_l_no_new_var_err_spec]
 
-lemma [sepref_fr_rules]:
-  \<open>((uncurry (return oo (check_extension_l_new_var_multiple_err_impl))),
-    uncurry (check_extension_l_new_var_multiple_err)) \<in> string_assn\<^sup>k *\<^sub>a poly_assn\<^sup>k \<rightarrow>\<^sub>a raw_string_assn\<close>
-   unfolding check_extension_l_new_var_multiple_err_impl_def
-     check_extension_l_new_var_multiple_err_def
-     list_assn_pure_conv
-   apply sepref_to_hoare
-   apply sep_auto
-   done
+definition check_extension_l_side_cond_err_imp :: \<open>_ \<Rightarrow> _\<close>  where
+  \<open>check_extension_l_side_cond_err_imp v p r s =
+    cl_to_clt ''Error while checking side conditions of extensions polynow, var is '' @ cl_to_clt v @
+    cl_to_clt '' polynomial is '' @ poly_print p @
+    cl_to_clt ''side condition p*p - p = '' @ poly_print s @ cl_to_clt '' and should be 0''\<close>
 
-sepref_register check_extension_l_dom_err fmlookup'
-  check_extension_l_side_cond_err check_extension_l_no_new_var_err
-  check_extension_l_new_var_multiple_err
+sepref_def check_extension_l_side_cond_err_impl is
+  \<open>uncurry3 (RETURN oooo check_extension_l_side_cond_err_imp)\<close>
+  :: \<open>strl_assn'\<^sup>k *\<^sub>a polynomial_assn\<^sup>k *\<^sub>a polynomial_assn\<^sup>k *\<^sub>a polynomial_assn\<^sup>k \<rightarrow>\<^sub>a strlt_assn\<close>
+  unfolding check_extension_l_side_cond_err_imp_def
+  by sepref
 
-sepref_register vars_of_poly_in
-  weak_equality_l
+lemma check_extension_l_side_cond_err_spec:
+  \<open>(uncurry3 (RETURN oooo check_extension_l_side_cond_err_imp),
+    uncurry3 check_extension_l_side_cond_err) \<in> Id \<rightarrow>\<^sub>f \<langle>Id\<rangle>nres_rel\<close>
+  apply (intro frefI nres_relI)
+  unfolding check_extension_l_side_cond_err_imp_def
+    check_extension_l_side_cond_err_def
+  by auto
 
-sepref_definition check_extension_l_impl
+lemmas check_extension_l_side_cond_err_hnr[sepref_fr_rules] =
+  check_extension_l_side_cond_err_impl.refine[FCOMP check_extension_l_side_cond_err_spec]
+
+definition check_extension_l_new_var_multiple_err_imp :: \<open>_ \<Rightarrow> _\<close>  where
+  \<open>check_extension_l_new_var_multiple_err_imp v p =
+    cl_to_clt ''Error while checking side conditions of extensions polynow, var is '' @ cl_to_clt v @
+    cl_to_clt '' but it either appears at least once in the polynomial or another new variable is created '' @
+    poly_print p @ cl_to_clt '' but should not.''\<close>
+
+sepref_def check_extension_l_new_var_multiple_err_impl is
+  \<open>uncurry (RETURN oo check_extension_l_new_var_multiple_err_imp)\<close>
+  :: \<open>strl_assn'\<^sup>k *\<^sub>a polynomial_assn\<^sup>k \<rightarrow>\<^sub>a strlt_assn\<close>
+  unfolding check_extension_l_new_var_multiple_err_imp_def
+  by sepref
+
+lemma check_extension_l_new_var_multiple_err_spec:
+  \<open>(uncurry (RETURN oo check_extension_l_new_var_multiple_err_imp),
+    uncurry check_extension_l_new_var_multiple_err) \<in> Id \<rightarrow>\<^sub>f \<langle>Id\<rangle>nres_rel\<close>
+  apply (intro frefI nres_relI)
+  unfolding check_extension_l_new_var_multiple_err_imp_def
+    check_extension_l_new_var_multiple_err_def
+  by auto
+
+lemmas check_extension_l_new_var_multiple_err_hnr[sepref_fr_rules] =
+  check_extension_l_new_var_multiple_err_impl.refine[FCOMP check_extension_l_new_var_multiple_err_spec]
+
+definition uminus_poly :: \<open>llist_polynomial \<Rightarrow> llist_polynomial\<close> where
+  \<open>uminus_poly p = map (\<lambda>(a,b). (a,-b)) p\<close>
+
+definition uminus_poly_nres :: \<open>llist_polynomial \<Rightarrow> llist_polynomial nres\<close> where
+  \<open>uminus_poly_nres = REC\<^sub>T (\<lambda>f p.
+    if p = [] then RETURN p
+    else do {
+      ((a,b), p) \<leftarrow> mop_list_pop_hd p;
+      r \<leftarrow> f p; RETURN ((a, -b) # r)
+    })\<close>
+
+lemma uminus_poly_nres_spec: \<open>uminus_poly_nres p = RETURN (uminus_poly p)\<close>
+  unfolding uminus_poly_nres_def uminus_poly_def
+proof (induction p)
+  case Nil
+  show ?case by (subst RECT_unfold, refine_mono) auto
+next
+  case (Cons x p)
+  show ?case
+    apply (subst RECT_unfold, refine_mono)
+    by (auto simp: Cons.IH split: prod.splits)
+qed
+
+sepref_register uminus_poly
+
+sepref_def uminus_poly_impl is \<open>uminus_poly_nres\<close>
+  :: \<open>polynomial_assn\<^sup>d \<rightarrow>\<^sub>a polynomial_assn\<close>
+  unfolding uminus_poly_nres_def
+  by sepref
+
+lemma uminus_poly_fref:
+  \<open>(uminus_poly_nres, RETURN o uminus_poly) \<in> Id \<rightarrow>\<^sub>f \<langle>Id\<rangle>nres_rel\<close>
+  by (intro frefI nres_relI) (auto simp: uminus_poly_nres_spec)
+
+lemmas uminus_poly_hnr[sepref_fr_rules] =
+  uminus_poly_impl.refine[FCOMP uminus_poly_fref]
+
+definition mnml_eq :: \<open>monomial_abs \<Rightarrow> monomial_abs \<Rightarrow> bool\<close> where
+  \<open>mnml_eq a b \<longleftrightarrow> a = b\<close>
+
+sepref_register mnml_eq
+
+lemma mnml_eq_op_hnr[sepref_fr_rules]:
+  \<open>(uncurry mnml_eq_impl', uncurry (RETURN oo mnml_eq))
+  \<in> monomial_assn\<^sup>k *\<^sub>a monomial_assn\<^sup>k \<rightarrow>\<^sub>a bool1_assn\<close>
+  unfolding mnml_eq_def by (rule mnml_eq_hnr)
+
+definition remove1_imp :: \<open>monomial_abs \<Rightarrow> llist_polynomial \<Rightarrow> llist_polynomial nres\<close> where
+  \<open>remove1_imp r cs \<equiv> REC\<^sub>T (\<lambda>f cs.
+    if cs=[] then RETURN cs
+    else doN {
+      (c,cs) \<leftarrow> mop_list_pop_hd cs;
+      if mnml_eq c r then
+        RETURN cs
+      else doN {
+        rs \<leftarrow> f cs;
+        RETURN (c#rs) 
+      }
+    }
+  ) cs\<close>
+
+lemma remove1_imp_spec:
+  \<open>remove1_imp r cs = RETURN (remove1 r cs)\<close>
+  unfolding remove1_imp_def
+proof (induction cs)
+  case Nil
+  show ?case by (subst RECT_unfold, refine_mono) auto
+next
+  case (Cons c cs)
+  show ?case
+    apply (subst RECT_unfold, refine_mono)
+    by (auto simp: mop_list_pop_hd_def mnml_eq_def Cons.IH pw_eq_iff refine_pw_simps)
+qed
+
+lemma remove1_imp_correct:
+  \<open>(RETURN oo remove1) = remove1_imp\<close>
+  by (intro ext) (simp add: remove1_imp_spec)
+
+term \<open>uncurry poly.cl_eq\<close>
+term \<open>uncurry (RETURN oo (=))\<close>
+sepref_def remove1_impl is \<open>uncurry (RETURN oo remove1)\<close>
+  :: \<open>monomial_assn\<^sup>k *\<^sub>a polynomial_assn\<^sup>d\<rightarrow>\<^sub>a polynomial_assn\<close>
+  unfolding remove1_imp_correct remove1_imp_def
+    ls_emp
+  apply sepref_dbg_keep
+  apply sepref_dbg_id_keep
+
+(* TODO: check if we could also make the string destructively alternatively *)
+lemma check_extension_l_alt:
+  \<open>check_extension_l spec A \<V> i v p = do {
+    let b = i \<notin># dom_m A \<and> v \<notin> \<V> \<and> ([COPY v], -1) \<in> set p;
+    if \<not>b
+    then do {
+      c \<leftarrow> check_extension_l_dom_err i;
+      RETURN (error_msg i c)
+    } else do {
+        p' \<leftarrow> remove1_imp ([COPY v], -1) p;
+        let b = vars_llist p' \<subseteq> \<V>;
+        if \<not>b
+        then do {
+          c \<leftarrow> check_extension_l_new_var_multiple_err v p';
+          RETURN (error_msg i c)
+        }
+        else do {
+           p2 \<leftarrow> mult_poly_full p' p';
+           let p' = map (\<lambda>(a,b). (a, -b)) p';
+           q \<leftarrow> add_poly_l p2 p';
+           eq \<leftarrow> weak_equality_l q [];
+           if eq then do {
+             RETURN (CSUCCESS)
+           } else do {
+            c \<leftarrow> check_extension_l_side_cond_err v p p' q;
+            RETURN (error_msg i c)
+          }
+        }
+      }
+    }\<close>
+  unfolding check_extension_l_def COPY_def
+  by simp
+
+thm remove1_impl.refine
+sepref_register remove1
+sepref_def check_extension_l_impl
   is \<open>uncurry5 check_extension_l\<close>
   :: \<open>polynomial_assn\<^sup>k *\<^sub>a polys_assn\<^sup>k *\<^sub>a vars_assn\<^sup>k *\<^sub>a si64_assn\<^sup>k *\<^sub>a strl_assn'\<^sup>k *\<^sub>a polynomial_assn\<^sup>k \<rightarrow>\<^sub>a
      status_assn\<close>
-  unfolding
-    check_extension_l_def
+  (* supply [[show_types]] *)
+  unfolding check_extension_l_alt
+    fmlookup'_def[symmetric]
+    in_dom_by_contains
+    vars_llist_alt_def
+    uminus_poly_def[symmetric]
   apply sepref_dbg_keep
+  apply sepref_dbg_trans_keep
+  apply sepref_dbg_trans_step_keep
+  apply sepref_dbg_side_unfold
+
   oops
 
-declare check_extension_l_impl.refine[sepref_fr_rules]
-
-sepref_definition check_del_l_impl
+sepref_def check_del_l_impl
   is \<open>uncurry2 check_del_l\<close>
-  :: \<open>poly_assn\<^sup>k *\<^sub>a polys_assn\<^sup>k *\<^sub>a uint64_nat_assn\<^sup>k \<rightarrow>\<^sub>a status_assn raw_string_assn\<close>
+  :: \<open>polynomial_assn\<^sup>k *\<^sub>a polys_assn\<^sup>k *\<^sub>a si64_assn\<^sup>k \<rightarrow>\<^sub>a status_assn\<close>
   supply [[goals_limit=1]]
   unfolding check_del_l_def
-    in_dom_m_lookup_iff
+    in_dom_by_contains
     fmlookup'_def[symmetric]
   by sepref
 
-lemmas [sepref_fr_rules] = check_del_l_impl.refine
-
 abbreviation pac_step_rel where
-  \<open>pac_step_rel \<equiv> p2rel (\<langle>Id, \<langle>monomial_rel\<rangle>list_rel, Id\<rangle> pac_step_rel_raw)\<close>
+  \<open>pac_step_rel \<equiv> p2rel (\<langle>Id, \<langle>Id\<rangle>list_rel, Id\<rangle> pac_step_rel_raw)\<close>
 
 sepref_register PAC_Polynomials_Operations.normalize_poly
   pac_src1 pac_src2 new_id pac_mult case_pac_step check_mult_l
   check_addition_l check_del_l check_extension_l
-
-lemma pac_step_rel_assn_alt_def2:
-  \<open>hn_ctxt (pac_step_rel_assn nat_assn poly_assn id_assn) b bi =
-       hn_val
-        (p2rel
-          (\<langle>nat_rel, poly_rel, Id :: (string \<times> _) set\<rangle>pac_step_rel_raw)) b bi\<close>
-  unfolding poly_assn_list hn_ctxt_def
-  by (induction nat_assn poly_assn \<open>id_assn :: string \<Rightarrow> _\<close> b bi rule: pac_step_rel_assn.induct)
-   (auto simp: p2rel_def hn_val_unfold pac_step_rel_raw.simps relAPP_def
-    pure_app_eq)
-
-
-lemma is_AddD_import[sepref_fr_rules]:
-  assumes \<open>CONSTRAINT is_pure K\<close>  \<open>CONSTRAINT is_pure V\<close>
-  shows
-    \<open>(return o pac_res, RETURN o pac_res) \<in> [\<lambda>x. is_Add x \<or> is_Mult x \<or> is_Extension x]\<^sub>a
-       (pac_step_rel_assn K V R)\<^sup>k \<rightarrow> V\<close>
-    \<open>(return o pac_src1, RETURN o pac_src1) \<in> [\<lambda>x. is_Add x \<or> is_Mult x \<or> is_Del x]\<^sub>a (pac_step_rel_assn K V R)\<^sup>k \<rightarrow> K\<close>
-    \<open>(return o new_id, RETURN o new_id) \<in> [\<lambda>x. is_Add x \<or> is_Mult x \<or> is_Extension x]\<^sub>a (pac_step_rel_assn K V R)\<^sup>k \<rightarrow> K\<close>
-    \<open>(return o is_Add, RETURN o is_Add) \<in>  (pac_step_rel_assn K V R)\<^sup>k \<rightarrow>\<^sub>a bool_assn\<close>
-    \<open>(return o is_Mult, RETURN o is_Mult) \<in> (pac_step_rel_assn K V R)\<^sup>k \<rightarrow>\<^sub>a bool_assn\<close>
-    \<open>(return o is_Del, RETURN o is_Del) \<in> (pac_step_rel_assn K V R)\<^sup>k \<rightarrow>\<^sub>a bool_assn\<close>
-    \<open>(return o is_Extension, RETURN o is_Extension) \<in> (pac_step_rel_assn K V R)\<^sup>k \<rightarrow>\<^sub>a bool_assn\<close>
-  using assms
-  by (sepref_to_hoare; sep_auto simp: pac_step_rel_assn_alt_def is_pure_conv ent_true_drop pure_app_eq
-      split: pac_step.splits; fail)+
-
-lemma [sepref_fr_rules]:
-  \<open>CONSTRAINT is_pure K \<Longrightarrow>
-  (return o pac_src2, RETURN o pac_src2) \<in> [\<lambda>x. is_Add x]\<^sub>a (pac_step_rel_assn K V R)\<^sup>k \<rightarrow> K\<close>
-  \<open>CONSTRAINT is_pure V \<Longrightarrow>
-  (return o pac_mult, RETURN o pac_mult) \<in> [\<lambda>x. is_Mult x]\<^sub>a (pac_step_rel_assn K V R)\<^sup>k \<rightarrow> V\<close>
-  \<open>CONSTRAINT is_pure R \<Longrightarrow>
-  (return o new_var, RETURN o new_var) \<in> [\<lambda>x. is_Extension x]\<^sub>a (pac_step_rel_assn K V R)\<^sup>k \<rightarrow> R\<close>
-  by (sepref_to_hoare; sep_auto simp: pac_step_rel_assn_alt_def is_pure_conv ent_true_drop pure_app_eq
-      split: pac_step.splits; fail)+
 
 lemma is_Mult_lastI:
   \<open>\<not> is_Add b \<Longrightarrow> \<not>is_Mult b \<Longrightarrow> \<not>is_Extension b \<Longrightarrow> is_Del b\<close>
@@ -953,36 +1163,17 @@ sepref_decl_intf ('k, 'b, 'lbl) apac_step is "('k, 'b, 'lbl) pac_step"
 
 sepref_register merge_cstatus full_normalize_poly new_var is_Add
 
-lemma poly_rel_the_pure:
-  \<open>poly_rel = the_pure poly_assn\<close> and
-  nat_rel_the_pure:
-  \<open>nat_rel = the_pure nat_assn\<close> and
- WTF_RF: \<open>pure (the_pure nat_assn) = nat_assn\<close>
-  unfolding poly_assn_list
-  by auto
-
-lemma [safe_constraint_rules]:
-    \<open>CONSTRAINT IS_LEFT_UNIQUE uint64_nat_rel\<close> and
-  single_valued_uint64_nat_rel[safe_constraint_rules]:
-    \<open>CONSTRAINT single_valued uint64_nat_rel\<close>
-  by (auto simp: IS_LEFT_UNIQUE_def single_valued_def uint64_nat_rel_def br_def)
-
-sepref_definition check_step_impl
+term pac_step_assn
+sepref_def check_step_impl
   is \<open>uncurry4 PAC_checker_l_step'\<close>
-  :: \<open>poly_assn\<^sup>k *\<^sub>a (status_assn raw_string_assn)\<^sup>d *\<^sub>a vars_assn\<^sup>d *\<^sub>a polys_assn\<^sup>d *\<^sub>a (pac_step_rel_assn (uint64_nat_assn) poly_assn (string_assn :: string \<Rightarrow> _))\<^sup>d \<rightarrow>\<^sub>a
-    status_assn raw_string_assn \<times>\<^sub>a vars_assn \<times>\<^sub>a polys_assn\<close>
-  supply [[goals_limit=1]] is_Mult_lastI[intro] single_valued_uint64_nat_rel[simp]
+  :: \<open>polynomial_assn\<^sup>k *\<^sub>a status_assn\<^sup>d *\<^sub>a vars_assn\<^sup>d *\<^sub>a polys_assn\<^sup>d *\<^sub>a pac_step_assn\<^sup>d
+  \<rightarrow>\<^sub>a status_assn \<times>\<^sub>a vars_assn \<times>\<^sub>a polys_assn\<close>
   unfolding PAC_checker_l_step_def PAC_checker_l_step'_def
     pac_step.case_eq_if Let_def
      is_success_alt_def[symmetric]
     uminus_poly_def[symmetric]
-    HOL_list.fold_custom_empty
-  by sepref
-
-
-declare check_step_impl.refine[sepref_fr_rules]
-
-sepref_register PAC_checker_l_step PAC_checker_l_step' fully_normalize_poly_impl
+  apply sepref_dbg_keep
+  oops
 
 definition PAC_checker_l' where
   \<open>PAC_checker_l' p \<V> A status steps = PAC_checker_l p (\<V>, A) status steps\<close>
@@ -992,46 +1183,49 @@ lemma PAC_checker_l_alt_def:
     (let (\<V>, A) = \<V>A in PAC_checker_l' p \<V> A status steps)\<close>
   unfolding PAC_checker_l'_def by auto
 
-sepref_definition PAC_checker_l_impl
+sepref_def PAC_checker_l_impl
   is \<open>uncurry4 PAC_checker_l'\<close>
-  :: \<open>poly_assn\<^sup>k *\<^sub>a vars_assn\<^sup>d *\<^sub>a polys_assn\<^sup>d *\<^sub>a (status_assn raw_string_assn)\<^sup>d *\<^sub>a
-       (list_assn (pac_step_rel_assn (uint64_nat_assn) poly_assn string_assn))\<^sup>k \<rightarrow>\<^sub>a
-     status_assn raw_string_assn \<times>\<^sub>a vars_assn \<times>\<^sub>a polys_assn\<close>
-  supply [[goals_limit=1]] is_Mult_lastI[intro]
+  :: \<open>polynomial_assn\<^sup>k *\<^sub>a vars_assn\<^sup>d *\<^sub>a polys_assn\<^sup>d *\<^sub>a status_assn \<^sup>d *\<^sub>a (cl_assn' pac_step_assn)\<^sup>k \<rightarrow>\<^sub>a
+     status_assn \<times>\<^sub>a vars_assn \<times>\<^sub>a polys_assn\<close>
   unfolding PAC_checker_l_def is_success_alt_def[symmetric] PAC_checker_l_step_alt_def
     nres_bind_let_law[symmetric] PAC_checker_l'_def
   apply (subst nres_bind_let_law)
+  apply sepref_dbg_keep
+  oops
+
+definition remap_polys_l_dom_err_imp :: \<open>_\<close>  where
+  \<open>remap_polys_l_dom_err_imp =
+    cl_to_clt ''Error during initialisation. Too many polynomials where provided. If this happens,'' @
+    cl_to_clt ''please report the example to the authors, because something went wrong during '' @
+    cl_to_clt ''code generation (code generation to arrays is likely to be broken).''\<close>
+
+sepref_def remap_polys_l_dom_err_impl is \<open>uncurry0 (RETURN remap_polys_l_dom_err_imp)\<close>
+  :: \<open>unit_assn\<^sup>k \<rightarrow>\<^sub>a strlt_assn\<close>
+  unfolding remap_polys_l_dom_err_imp_def
   by sepref
 
-declare PAC_checker_l_impl.refine[sepref_fr_rules]
+lemma remap_polys_l_dom_err_fref:
+  \<open>(uncurry0 (RETURN remap_polys_l_dom_err_imp), uncurry0 remap_polys_l_dom_err)
+  \<in> unit_rel \<rightarrow>\<^sub>f \<langle>Id\<rangle>nres_rel\<close>
+  unfolding remap_polys_l_dom_err_imp_def remap_polys_l_dom_err_def cl_to_clt_id
+  apply auto
+  oops
+
+lemmas remap_polys_l_dom_err_hnr[sepref_fr_rules] =
+  remapt_polys_l_dom_err_impl.refine[FCOMP remap_polys_l_dom_err_fref]
+
+lemma pow_2_64: \<open>(2::nat) ^ 64 = 18446744073709551616\<close>
+  by auto
 
 abbreviation polys_assn_input where
   \<open>polys_assn_input \<equiv> iam_fmap_assn nat_assn poly_assn\<close>
 
-definition remap_polys_l_dom_err_impl :: \<open>_\<close>  where
-  \<open>remap_polys_l_dom_err_impl =
-    ''Error during initialisation. Too many polynomials where provided. If this happens,'' @
-    ''please report the example to the authors, because something went wrong during '' @
-    ''code generation (code generation to arrays is likely to be broken).''\<close>
-
-lemma [sepref_fr_rules]:
-  \<open>((uncurry0 (return (remap_polys_l_dom_err_impl))),
-    uncurry0 (remap_polys_l_dom_err)) \<in> unit_assn\<^sup>k \<rightarrow>\<^sub>a raw_string_assn\<close>
-   unfolding remap_polys_l_dom_err_def
-     remap_polys_l_dom_err_def
-     list_assn_pure_conv
-   by sepref_to_hoare sep_auto
-
-text \<open>MLton is not able to optimise the calls to pow.\<close>
-lemma pow_2_64: \<open>(2::nat) ^ 64 = 18446744073709551616\<close>
-  by auto
-
 sepref_register upper_bound_on_dom op_fmap_empty
 
-sepref_definition remap_polys_l_impl
+sepref_def remap_polys_l_impl
   is \<open>uncurry2 remap_polys_l2\<close>
-  :: \<open>poly_assn\<^sup>k *\<^sub>a vars_assn\<^sup>d *\<^sub>a polys_assn_input\<^sup>d \<rightarrow>\<^sub>a
-    status_assn raw_string_assn \<times>\<^sub>a vars_assn \<times>\<^sub>a polys_assn\<close>
+  :: \<open>polynomial_assn\<^sup>k *\<^sub>a vars_assn\<^sup>d *\<^sub>a polys_assn_input\<^sup>d \<rightarrow>\<^sub>a
+    status_assn \<times>\<^sub>a vars_assn \<times>\<^sub>a polys_assn\<close>
   supply [[goals_limit=1]] is_Mult_lastI[intro] indom_mI[dest]
   unfolding remap_polys_l2_def op_fmap_empty_def[symmetric] while_eq_nfoldli[symmetric]
     while_upt_while_direct pow_2_64
@@ -1051,96 +1245,40 @@ lemma remap_polys_l2_remap_polys_l:
 
 lemma [sepref_fr_rules]:
    \<open>(uncurry2 remap_polys_l_impl,
-     uncurry2 remap_polys_l) \<in> poly_assn\<^sup>k *\<^sub>a vars_assn\<^sup>d *\<^sub>a polys_assn_input\<^sup>d \<rightarrow>\<^sub>a
-       status_assn raw_string_assn \<times>\<^sub>a vars_assn \<times>\<^sub>a polys_assn\<close>
+     uncurry2 remap_polys_l) \<in> polynomial_assn\<^sup>k *\<^sub>a vars_assn\<^sup>d *\<^sub>a polys_assn_input\<^sup>d \<rightarrow>\<^sub>a
+       status_assn \<times>\<^sub>a vars_assn \<times>\<^sub>a polys_assn\<close>
    using hfcomp_tcomp_pre[OF remap_polys_l2_remap_polys_l remap_polys_l_impl.refine]
    by (auto simp: hrp_comp_def hfprod_def)
 
 sepref_register remap_polys_l
 
-sepref_definition full_checker_l_impl
+sepref_def full_checker_l_impl
   is \<open>uncurry2 full_checker_l\<close>
-  :: \<open>poly_assn\<^sup>k *\<^sub>a polys_assn_input\<^sup>d *\<^sub>a (list_assn (pac_step_rel_assn (uint64_nat_assn) poly_assn string_assn))\<^sup>k \<rightarrow>\<^sub>a
-    status_assn raw_string_assn \<times>\<^sub>a vars_assn \<times>\<^sub>a polys_assn\<close>
+  :: \<open>polynomial_assn\<^sup>d *\<^sub>a polys_assn_input\<^sup>d *\<^sub>a (cl_assn' pac_step_assn)\<^sup>d \<rightarrow>\<^sub>a
+    status_assn \<times>\<^sub>a vars_assn \<times>\<^sub>a polys_assn\<close>
   supply [[goals_limit=1]] is_Mult_lastI[intro]
   unfolding full_checker_l_def hs.fold_custom_empty
     union_vars_poly_alt_def[symmetric]
     PAC_checker_l_alt_def
   by sepref
 
-sepref_definition PAC_update_impl
+sepref_def PAC_update_impl
   is \<open>uncurry2 (RETURN ooo fmupd)\<close>
-  :: \<open>nat_assn\<^sup>k *\<^sub>a poly_assn\<^sup>k *\<^sub>a (polys_assn_input)\<^sup>d \<rightarrow>\<^sub>a polys_assn_input\<close>
+  :: \<open>nat_assn\<^sup>k *\<^sub>a poly_assn\<^sup>k *\<^sub>a polys_assn_input\<^sup>d \<rightarrow>\<^sub>a polys_assn_input\<close>
   unfolding comp_def
   by sepref
 
-sepref_definition PAC_empty_impl
+sepref_def PAC_empty_impl
   is \<open>uncurry0 (RETURN fmempty)\<close>
   :: \<open>unit_assn\<^sup>k \<rightarrow>\<^sub>a polys_assn_input\<close>
   unfolding op_iam_fmap_empty_def[symmetric] pat_fmap_empty
   by sepref
 
-sepref_definition empty_vars_impl
+sepref_def empty_vars_impl
   is \<open>uncurry0 (RETURN {})\<close>
   :: \<open>unit_assn\<^sup>k \<rightarrow>\<^sub>a vars_assn\<close>
   unfolding hs.fold_custom_empty
   by sepref
-
-text \<open>This is a hack for performance. There is no need to recheck that that a char is valid when
-  working on chars coming from strings... It is not that important in most cases, but in our case
-  the preformance difference is really large.\<close>
-
-
-definition unsafe_asciis_of_literal :: \<open>_\<close> where
-  \<open>unsafe_asciis_of_literal xs = String.asciis_of_literal xs\<close>
-
-definition unsafe_asciis_of_literal' :: \<open>_\<close> where
-  [simp, symmetric, code]: \<open>unsafe_asciis_of_literal' = unsafe_asciis_of_literal\<close>
-
-code_printing
-  constant unsafe_asciis_of_literal' \<rightharpoonup>
-    (SML) "!(List.map (fn c => let val k = Char.ord c in IntInf.fromInt k end) /o String.explode)"
-
-text \<open>
-  Now comes the big and ugly and unsafe hack.
-
-  Basically, we try to avoid the conversion to IntInf when calculating the hash. The performance
-  gain is roughly 40\%, which is a LOT and definitively something we need to do. We are aware that the
-  SML semantic encourages compilers to optimise conversions, but this does not happen here,
-  corroborating our early observation on the verified SAT solver IsaSAT.x
-\<close>
-definition raw_explode where
-  [simp]: \<open>raw_explode = String.explode\<close>
-code_printing
-  constant raw_explode \<rightharpoonup>
-    (SML) "String.explode"
-
-definition \<open>hashcode_literal' s \<equiv>
-    foldl (\<lambda>h x. h * 33 + uint32_of_int (of_char x)) 5381
-     (raw_explode s)\<close>
-
-definition uint32_of_char :: \<open>char \<Rightarrow> uint32\<close>
-  where [code_abbrev]: \<open>uint32_of_char x = uint32_of_int (int_of_char x)\<close>
-
-code_printing
-  constant uint32_of_char \<rightharpoonup>
-    (SML) "!(Word32.fromInt /o (Char.ord))"
-
-lemma [code]: \<open>hashcode s = hashcode_literal' s\<close>
-  unfolding hashcode_literal_def hashcode_list_def
-  apply (auto simp: unsafe_asciis_of_literal_def hashcode_list_def
-     String.asciis_of_literal_def hashcode_literal_def hashcode_literal'_def)
-  done
-
-text \<open>We compile Pastèque in \<^file>\<open>PAC_Checker_MLton.thy\<close>.\<close>
-export_code PAC_checker_l_impl PAC_update_impl PAC_empty_impl the_error is_cfailed is_cfound
-  int_of_integer Del Add Mult nat_of_integer String.implode remap_polys_l_impl
-  fully_normalize_poly_impl union_vars_poly_impl empty_vars_impl
-  full_checker_l_impl check_step_impl CSUCCESS
-  Extension hashcode_literal' version
-  in SML_imp module_name PAC_Checker
-
-
 section \<open>Correctness theorem\<close>
 
 context poly_embed
