PAC_Checker_LLVM/PAC_Checker_Relation.thy
@@ -30,21 +30,6 @@ sepref_def mnl_le_impl is \<open>uncurry (RETURN oo mnl_le)\<close>
   unfolding mnl_le_def
   by sepref
 
-sepref_def poly_merge_impl is \<open>uncurry (RETURN oo merge_mnls)\<close>
-  :: \<open>poly_assn\<^sup>d *\<^sub>a poly_assn\<^sup>d \<rightarrow>\<^sub>a poly_assn\<close>
-  unfolding merge_mnls_def merge_RECT
-  by sepref
-
-sepref_def poly_split_impl is \<open>RETURN o alt_split\<close>
-  :: \<open>poly_assn\<^sup>d \<rightarrow>\<^sub>a poly_assn \<times>\<^sub>a poly_assn\<close>
-  unfolding alt_split_RECT_ol
-  by sepref
-
-sepref_def poly_msort_impl is \<open>RETURN o msort_mnls\<close>
-  :: \<open>poly_assn\<^sup>d \<rightarrow>\<^sub>a poly_assn\<close>
-  unfolding msort_mnls_def msort_alt_RECT merge_mnls_def[symmetric]
-  by sepref
-
 text \<open>Correctness at the abstract level: multiset preservation and sortedness w.r.t.
   the (weak) monomial order on pairs \<emdash> the ingredients for \<open>sort_poly_spec\<close>.\<close>
 
@@ -71,12 +56,6 @@ lemma term_order_rel_alt_def:
   apply (rule arg_cong[where f=lexord])
   by (auto simp: p2rel_def char.lexordp_conv_lexord less_than_char_def)
 
-text \<open>The \<open>list :: linorder\<close> instantiation (\<open>less_list = lexordp (<)\<close>,
-  \<open>less_eq_list = lexordp_eq\<close>) has moved upstream to \<open>String_Assn\<close> so that the
-  refinement rule for \<open>strl_lt\<close> can be stated against \<open>(<)\<close>; it is inherited here
-  via \<open>Monom_Assn\<close>.\<close>
-
-
 lemma term_order_rel'_alt_def_lexord:
     \<open>term_order_rel' x y = ord_class.lexordp x y\<close> and
   term_order_rel'_alt_def:
@@ -87,7 +66,7 @@ proof -
     \<open>term_order_rel' x y \<longleftrightarrow> x < y\<close>
     by (auto simp: lexordp_conv_lexord less_eq_list_def
          less_list_def lexordp_def var_order_rel_def
-         rel2p_def term_order_rel_alt_def p2rel_def)
+         rel2p_def term_order_rel_alt_def p2rel_def less_char_inst)
 qed
 
 definition string2_rel :: \<open>(string \<times> string) set\<close> where
@@ -95,8 +74,7 @@ definition string2_rel :: \<open>(string \<times> string) set\<close> where
 
 lemma char_of_word_less_iff: \<open>char_of_word a < char_of_word b \<longleftrightarrow> (a :: 8 word) < b\<close>
   using unat_of_char_mod
-  by (auto simp: char_of_word_def word_less_nat_alt PAC_Polynomials_Term.less_char_def
-      simp flip: less_char_def)
+  by (auto simp: char_of_word_def word_less_nat_alt less_char_inst less_char_def)
 
 lemma lexord_char_rel_mono_iff:
   assumes \<open>(xs, xs') \<in> \<langle>char_rel\<rangle>list_rel\<close> and
@@ -118,97 +96,97 @@ next
     
 qed
 
-lemma list_rel_list_rel_order_iff:
-  assumes \<open>(a, b) \<in> \<langle>string_rel\<rangle>list_rel\<close> \<open>(a', b') \<in> \<langle>string_rel\<rangle>list_rel\<close>
-  shows \<open>a < a' \<longleftrightarrow> b < b'\<close>
-proof
-  have H: \<open>(a, b) \<in> \<langle>string_rel\<rangle>list_rel \<Longrightarrow>
-       (a, cs) \<in> \<langle>string_rel\<rangle>list_rel \<Longrightarrow> b = cs\<close> for cs
-     using single_valued_monom_rel' IS_RIGHT_UNIQUE_string_rel
-     unfolding string2_rel_def
-     by (subst (asm)list_rel_sv_iff[symmetric])
-       (auto simp: single_valued_def)
-  assume \<open>a < a'\<close>
-  then consider
-    u u' where \<open>a' = a @ u # u'\<close> |
-    u aa v w aaa where \<open>a = u @ aa # v\<close> \<open>a' = u @ aaa # w\<close> \<open>aa < aaa\<close>
-    by (subst (asm) less_list_def)
-     (auto simp: lexord_def List.lexordp_def
-      list_rel_append1 list_rel_split_right_iff)
-  then show \<open>b < b'\<close>
-  proof cases
-    case 1
-    then show \<open>b < b'\<close>
-      using assms
-      by (subst less_list_def)
-        (auto simp: lexord_def List.lexordp_def
-        list_rel_append1 list_rel_split_right_iff dest: H)
-  next
-    case 2
-    then obtain u' aa' v' w' aaa' where
-       \<open>b = u' @ aa' # v'\<close> \<open>b' = u' @ aaa' # w'\<close>
-       \<open>(aa, aa') \<in> string_rel\<close>
-       \<open>(aaa, aaa') \<in> string_rel\<close>
-      using assms
-      by (smt (verit) list_rel_append1 list_rel_split_right_iff single_valued_def single_valued_monom_rel)
-    have aa_lex: \<open>(aa, aaa) \<in> lexord {(x, y). x < y}\<close>
-      using \<open>aa < aaa\<close> unfolding less_list_def lexordp_conv_lexord
-      using List.lexordp_def by blast
-    have \<open>aa' < aaa'\<close>
-      unfolding less_list_def lexordp_conv_lexord
-      using lexord_char_rel_mono_iff[OF \<open>(aa, aa') \<in> string_rel\<close>[unfolded string_rel_def]
-          \<open>(aaa, aaa') \<in> string_rel\<close>[unfolded string_rel_def]] aa_lex
-      using List.lexordp_def by blast
-    then show \<open>b < b'\<close>
-      using \<open>b = u' @ aa' # v'\<close> \<open>b' = u' @ aaa' # w'\<close>
-      by (subst less_list_def)
-        (fastforce simp: lexord_def List.lexordp_def
-        list_rel_append1 list_rel_split_right_iff)
-  qed
-next
-  have H: \<open>(a, b) \<in> \<langle>string_rel\<rangle>list_rel \<Longrightarrow>
-       (a', b) \<in> \<langle>string_rel\<rangle>list_rel \<Longrightarrow> a = a'\<close> for a a' b
-     using single_valued_monom_rel'
-     by (auto simp: single_valued_def IS_LEFT_UNIQUE_def
-       simp flip: inv_list_rel_eq)
-  assume \<open>b < b'\<close>
-  then consider
-    u u' where \<open>b' = b @ u # u'\<close> |
-    u aa v w aaa where \<open>b = u @ aa # v\<close> \<open>b' = u @ aaa # w\<close> \<open>aa < aaa\<close>
-    by (subst (asm) less_list_def)
-     (auto simp: lexord_def List.lexordp_def
-      list_rel_append1 list_rel_split_right_iff)
-  then show \<open>a < a'\<close>
-  proof cases
-    case 1
-    then show \<open>a < a'\<close>
-      using assms
-      by (subst less_list_def)
-        (auto simp: lexord_def List.lexordp_def
-        list_rel_append2 list_rel_split_left_iff dest: H)
-  next
-    case 2
-    then obtain u' aa' v' w' aaa' where
-       \<open>a = u' @ aa' # v'\<close> \<open>a' = u' @ aaa' # w'\<close>
-       \<open>(aa', aa) \<in> string_rel\<close>
-       \<open>(aaa', aaa) \<in> string_rel\<close>
-      using assms
-      by (auto simp: lexord_def List.lexordp_def
-        list_rel_append2 list_rel_split_left_iff dest: H)
-    have aa_lex: \<open>(aa, aaa) \<in> lexord {(x, y). x < y}\<close>
-      using \<open>aa < aaa\<close> unfolding less_list_def lexordp_conv_lexord
-      using List.lexordp_def by blast
-    have \<open>aa' < aaa'\<close>
-      unfolding less_list_def lexordp_conv_lexord
-      using lexord_char_rel_mono_iff[OF \<open>(aa', aa) \<in> string_rel\<close>[unfolded string_rel_def]
-          \<open>(aaa', aaa) \<in> string_rel\<close>[unfolded string_rel_def]] aa_lex
-      using List.lexordp_def by blast
-    then show \<open>a < a'\<close>
-      using \<open>a = u' @ aa' # v'\<close> \<open>a' = u' @ aaa' # w'\<close>
-      by (subst less_list_def)
-        (fastforce simp: lexord_def List.lexordp_def
-        list_rel_append1 list_rel_split_right_iff)
-  qed
-qed
+(* lemma list_rel_list_rel_order_iff:
+ *   assumes \<open>(a, b) \<in> \<langle>string_rel\<rangle>list_rel\<close> \<open>(a', b') \<in> \<langle>string_rel\<rangle>list_rel\<close>
+ *   shows \<open>a < a' \<longleftrightarrow> b < b'\<close>
+ * proof
+ *   have H: \<open>(a, b) \<in> \<langle>string_rel\<rangle>list_rel \<Longrightarrow>
+ *        (a, cs) \<in> \<langle>string_rel\<rangle>list_rel \<Longrightarrow> b = cs\<close> for cs
+ *      using single_valued_monom_rel' IS_RIGHT_UNIQUE_string_rel
+ *      unfolding string2_rel_def
+ *      by (subst (asm)list_rel_sv_iff[symmetric])
+ *        (auto simp: single_valued_def)
+ *   assume \<open>a < a'\<close>
+ *   then consider
+ *     u u' where \<open>a' = a @ u # u'\<close> |
+ *     u aa v w aaa where \<open>a = u @ aa # v\<close> \<open>a' = u @ aaa # w\<close> \<open>aa < aaa\<close>
+ *     by (subst (asm) less_list_def)
+ *      (auto simp: lexord_def List.lexordp_def
+ *       list_rel_append1 list_rel_split_right_iff)
+ *   then show \<open>b < b'\<close>
+ *   proof cases
+ *     case 1
+ *     then show \<open>b < b'\<close>
+ *       using assms
+ *       by (subst less_list_def)
+ *         (auto simp: lexord_def List.lexordp_def
+ *         list_rel_append1 list_rel_split_right_iff dest: H)
+ *   next
+ *     case 2
+ *     then obtain u' aa' v' w' aaa' where
+ *        \<open>b = u' @ aa' # v'\<close> \<open>b' = u' @ aaa' # w'\<close>
+ *        \<open>(aa, aa') \<in> string_rel\<close>
+ *        \<open>(aaa, aaa') \<in> string_rel\<close>
+ *       using assms
+ *       by (smt (verit) list_rel_append1 list_rel_split_right_iff single_valued_def single_valued_monom_rel)
+ *     have aa_lex: \<open>(aa, aaa) \<in> lexord {(x, y). x < y}\<close>
+ *       using \<open>aa < aaa\<close> unfolding less_list_def lexordp_conv_lexord
+ *       using List.lexordp_def by blast
+ *     have \<open>aa' < aaa'\<close>
+ *       unfolding less_list_def lexordp_conv_lexord
+ *       using lexord_char_rel_mono_iff[OF \<open>(aa, aa') \<in> string_rel\<close>[unfolded string_rel_def]
+ *           \<open>(aaa, aaa') \<in> string_rel\<close>[unfolded string_rel_def]] aa_lex
+ *       using List.lexordp_def by blast
+ *     then show \<open>b < b'\<close>
+ *       using \<open>b = u' @ aa' # v'\<close> \<open>b' = u' @ aaa' # w'\<close>
+ *       by (subst less_list_def)
+ *         (fastforce simp: lexord_def List.lexordp_def
+ *         list_rel_append1 list_rel_split_right_iff)
+ *   qed
+ * next
+ *   have H: \<open>(a, b) \<in> \<langle>string_rel\<rangle>list_rel \<Longrightarrow>
+ *        (a', b) \<in> \<langle>string_rel\<rangle>list_rel \<Longrightarrow> a = a'\<close> for a a' b
+ *      using single_valued_monom_rel'
+ *      by (auto simp: single_valued_def IS_LEFT_UNIQUE_def
+ *        simp flip: inv_list_rel_eq)
+ *   assume \<open>b < b'\<close>
+ *   then consider
+ *     u u' where \<open>b' = b @ u # u'\<close> |
+ *     u aa v w aaa where \<open>b = u @ aa # v\<close> \<open>b' = u @ aaa # w\<close> \<open>aa < aaa\<close>
+ *     by (subst (asm) less_list_def)
+ *      (auto simp: lexord_def List.lexordp_def
+ *       list_rel_append1 list_rel_split_right_iff)
+ *   then show \<open>a < a'\<close>
+ *   proof cases
+ *     case 1
+ *     then show \<open>a < a'\<close>
+ *       using assms
+ *       by (subst less_list_def)
+ *         (auto simp: lexord_def List.lexordp_def
+ *         list_rel_append2 list_rel_split_left_iff dest: H)
+ *   next
+ *     case 2
+ *     then obtain u' aa' v' w' aaa' where
+ *        \<open>a = u' @ aa' # v'\<close> \<open>a' = u' @ aaa' # w'\<close>
+ *        \<open>(aa', aa) \<in> string_rel\<close>
+ *        \<open>(aaa', aaa) \<in> string_rel\<close>
+ *       using assms
+ *       by (auto simp: lexord_def List.lexordp_def
+ *         list_rel_append2 list_rel_split_left_iff dest: H)
+ *     have aa_lex: \<open>(aa, aaa) \<in> lexord {(x, y). x < y}\<close>
+ *       using \<open>aa < aaa\<close> unfolding less_list_def lexordp_conv_lexord
+ *       using List.lexordp_def by blast
+ *     have \<open>aa' < aaa'\<close>
+ *       unfolding less_list_def lexordp_conv_lexord
+ *       using lexord_char_rel_mono_iff[OF \<open>(aa', aa) \<in> string_rel\<close>[unfolded string_rel_def]
+ *           \<open>(aaa', aaa) \<in> string_rel\<close>[unfolded string_rel_def]] aa_lex
+ *       using List.lexordp_def by blast
+ *     then show \<open>a < a'\<close>
+ *       using \<open>a = u' @ aa' # v'\<close> \<open>a' = u' @ aaa' # w'\<close>
+ *       by (subst less_list_def)
+ *         (fastforce simp: lexord_def List.lexordp_def
+ *         list_rel_append1 list_rel_split_right_iff)
+ *   qed
+ * qed *)
 
 end
